comp1_type done

basic_types.v
@@ -3,3 +3,17 @@ From mathcomp Require Import ssreflect seq ssrnat.
 From istari Require Import Sigma Tactics
      Syntax Subst SimpSub Promote Hygiene
      ContextHygiene Equivalence Rules Defined.
+
+Definition oof M A: (@Syntax.judgement False) := deq M M A.
+
+Definition oof_t M: (@Syntax.judgement False) := deqtype M M.
+
+Lemma zero_typed: forall G,
+    tr G (oof nzero nattp). Admitted.
+
+Lemma leq_refl: forall G n,
+    tr G (deq n n nattp) ->
+    tr G (oof triv (leqpagetp n n)). Admitted.
+
+Hint Resolve zero_typed.
+Hint Resolve leq_refl.
